verif/verif_isvalid.v
@@ -1,0 +1,37 @@
+(** * verif_isvalid.v : Correctness proof of isValid, isFirst and RL_CursorIsValid *)
+
+Require Import VST.floyd.proofauto.
+Require Import VST.floyd.library.
+Require Import relation_mem.
+Instance CompSpecs : compspecs. make_compspecs prog. Defined.
+Definition Vprog : varspecs. mk_varspecs prog. Defined.
+
+Require Import VST.msl.wand_frame.
+Require Import VST.msl.iter_sepcon.
+Require Import VST.floyd.reassoc_seq.
+Require Import VST.floyd.field_at_wand.
+Require Import FunInd.
+Require Import btrees.
+Require Import btrees_sep.
+Require Import btrees_spec.
+Require Import verif_currnode.
+Require Import verif_entryindex.
+
+Lemma body_isValid: semax_body Vprog Gprog f_isValid isValid_spec.
+Proof.
+  start_function.
+  (* need to prove entryIndex and currNode first *)
+Admitted.
+
+Lemma body_RL_CursorIsValid: semax_body Vprog Gprog f_RL_CursorIsValid RL_CursorIsValid_spec.
+Proof.
+  start_function.
+  (* need to prove entryIndex and currNode first *)
+Admitted.
+
+Lemma body_isFirst: semax_body Vprog Gprog f_isFirst isFirst_spec.
+Proof.
+  start_function.
+  (* need to prove entryIndex and currNode first *)
+Admitted.
+ 
